examples/contractMorphisms/upgradeable/upgradeable.v
@@ -5,6 +5,7 @@ From ConCert.Execution Require Import Monad.
 From ConCert.Execution Require Import ResultMonad.
 From ConCert.Execution Require Import Serializable.
 From ConCert.Execution Require Import ContractMorphisms.
+From ConCert.Execution Require Import ContractSystems.
 From ConCert.Utils Require Import RecordUpdate.
 From ConCert.Utils Require Import Extras.
 From Coq Require Import Ensembles.
@@ -20,37 +21,65 @@ Open Scope N_scope.
 Open Scope string.
 
 (* the upgradeable example *)
-
-Section UpgradeableContract.
+Section Upgradeable.
 Context { Base : ChainBase }.
 Set Primitive Projections.
 Set Nonrecursive Elimination Schemes.
 
-(* contract types definition *)
+(** Goal: 
+    - A family of versioned contracts C_f : for all version v, C_f v
+    - Forall v, C_f v -> C -> C_b which decomposes the upgradeability structure of C
+*)
+
+Section ContractDefinitions.
+(*** Contract types definition *)
+(** Main contract C *)
 Inductive entrypoint := 
-    | next (u : unit)
-    | upgrade_fun (s' : N -> N).
-Record storage := build_storage {
-    n : N ; 
-    s : N -> N ; }.
+| next (u : unit)
+| upgrade_fun (s' : N -> N).
+Record storage := { n : N ; s : N -> N ; }.
 Definition setup := storage.
 Definition error := N.
 Definition result : Type := ResultMonad.result (storage * list ActionBody) error.
 
-(* derive serializable typeclass *)
+(** Skeleton contract C_skel (to be C_b) *)
+Inductive entrypoint_skel := 
+| upgrade_fun_b (s' : N -> N).
+Record storage_b := { s_b : N -> N ; }.
+Definition setup_b := storage_b.
+Definition error_b := N.
+Definition result_b : Type := ResultMonad.result (storage_b * list ActionBody) error_b.
+
+(** Version contracts C_f v, for v : storage_b *)
+Inductive entrypoint_version := | next_f (u : unit).
+Record storage_version := { n_f : N }.
+Definition entrypoint_f : storage_b -> Type := fun v => entrypoint_version.
+Definition storage_f    : storage_b -> Type := fun v => storage_version.
+Definition setup_f      : storage_b -> Type := fun v => N.
+Definition error_f      : storage_b -> Type := fun v => N.
+Definition result_f     : storage_b -> Type := 
+    fun v => ResultMonad.result ((storage_f v) * list ActionBody) (error_f v).
+
 Section Serialization.
     Global Instance storage_serializable : Serializable storage := todo "".
     Global Instance entrypoint_serializable : Serializable entrypoint := todo "".
+    Global Instance storage_s_serializable : Serializable storage_b := todo "".
+    Global Instance entrypoint_s_serializable : Serializable entrypoint_skel := todo "".
+    Global Instance storage_f_serializable : forall v, Serializable (storage_f v) := todo "".
+    Global Instance entrypoint_f_serializable : forall v, Serializable (entrypoint_f v) := todo "".
 End Serialization.
 
-(* init function definition *)
+(** Contract, init, and receive definitions *)
+
+(** Main contract C *)
+(* init *)
 Definition init (_ : Chain)
                 (_ : ContractCallContext)
                 (init_state : setup)
                 : ResultMonad.result storage N := 
     Ok (init_state).
 
-(* receive function definition *)
+(* receive *)
 Definition receive (_ : Chain)
                 (_ : ContractCallContext)
                 (storage : storage)
@@ -66,230 +95,272 @@ Definition receive (_ : Chain)
     | None => Err 0
     end.
 
-(* construct the contract *)
+(* the contract C *)
 Definition C : Contract setup entrypoint storage error := 
     build_contract init receive.
 
-End UpgradeableContract.
-
-
-Section SkeletonContract.
-Context { Base : ChainBase }.
-
-(* contract types definition *)
-Definition setup_s := unit.
-Inductive entrypoint_s := 
-    | next_s (u : unit)
-    | upgrade_fun_s (s' : N -> N).
-Record storage_s := build_storage_s { n_s : N ; s_s : N -> N ; }.
-Definition error_s := N.
-Definition result_s : Type := ResultMonad.result (storage_s * list ActionBody) error_s.
-
-(* derive serializable typeclass *)
-Section Serialization.
-    Global Instance storage_s_serializable : Serializable storage_s := todo "".
-    Global Instance entrypoint_s_serializable : Serializable entrypoint_s := todo "".
-End Serialization.
-
-(* init function definition *)
-Definition init_s (_ : Chain)
+(** Skeleton Contract (to be the base contract) *)
+(* init *)
+Definition init_skel (_ : Chain)
                 (_ : ContractCallContext)
-                (_ : setup_s)
-                : ResultMonad.result storage_s N := 
-    let storage_s := {|
-        n_s := 0 ; 
-        s_s := (fun (n : N) => 0) ; |} in 
-    Ok (storage_s).
+                (init_state_b : setup_b)
+                : ResultMonad.result storage_b N := 
+    Ok (init_state_b).
 
-(* receive function definition *)
-Definition receive_s (_ : Chain)
+(* receive *)
+Definition receive_skel (_ : Chain)
                 (_ : ContractCallContext)
-                (storage_s : storage_s)
-                (msg : option entrypoint_s)
-                : result_s :=
+                (_ : storage_b)
+                (msg : option entrypoint_skel)
+                : result_b :=
     match msg with 
-    | Some (next_s _) => 
-        let st := {| n_s := storage_s.(s_s) storage_s.(n_s) ; s_s := storage_s.(s_s) ; |} in 
+    | Some (upgrade_fun_b s_new) => 
+        let st := {| s_b := s_new ; |} in 
         Ok (st, [])
-    | Some (upgrade_fun_s _) => Ok (storage_s, [])
     | None => Err 0
     end.
 
-(* construct the contract *)
-Definition C_s : Contract setup_s entrypoint_s storage_s error_s := 
-    build_contract init_s receive_s.
+(* the contract C_skel *)
+Definition C_skel : Contract setup_b entrypoint_skel storage_b error_b :=
+    build_contract init_skel receive_skel.
 
-End SkeletonContract.
+(** For the morphisms, we define the base contract *)
+Definition C_b := pointed_contract C_skel.
+Definition entrypoint_b := (entrypoint_skel + unit)%type.
 
-Section Projection.
-Context { Base : ChainBase }.
 
-(* using the simple morphism construction *)
-Definition msg_morph (e : entrypoint) : entrypoint_s := 
-    match e with 
-    | next _ => next_s tt 
-    | upgrade_fun s' => upgrade_fun_s s'
+(** The family of version contracts C_f *)
+(* init *)
+Definition init_f (version : storage_b)
+                (_ : Chain)
+                (_ : ContractCallContext)
+                (n : setup_f version)
+                : ResultMonad.result (storage_f version) (error_f version) := 
+    let storage_f := {| n_f := n ; |} in 
+    Ok (storage_f).
+
+(* receive *)
+Definition receive_f (version : storage_b)
+                (_ : Chain)
+                (_ : ContractCallContext)
+                (storage_f : storage_f version)
+                (msg : option (entrypoint_f version))
+                : result_f version :=
+    match msg with 
+    | Some (next_f _) => 
+        let st := {| n_f := version.(s_b) storage_f.(n_f) ; |} in 
+        Ok (st, [])
+    | None => Err 0
     end.
-Definition setup_morph : setup -> setup_s := (fun (_ : setup) => tt).
-Definition state_morph (st : storage) : storage_s := 
-    {| n_s := 0 ; s_s := (fun (n : N) => 0) ; |}.
-    (* {| n_s := st.(n) ; s_s := st.(s) |}. *)
-Definition error_morph : error -> error_s := id.
+
+(* the contract C_f *)
+Definition C_f (version : storage_b) : Contract (setup_f version) (entrypoint_f version) (storage_f version) (error_f version) := 
+    build_contract (init_f version) (receive_f version).
+
+End ContractDefinitions.
+
+
+(** Define the contract morphisms  *)
+Section Morphisms.
+
+(** f_p : C ->> C_b *)
+Section Quotient.
+Definition zero_fn : N -> N := (fun (x : N) => 0).
+Definition null_storage_b : storage_b := {| s_b := zero_fn |}.
+Definition null_setup_b : setup_b := {| s_b := zero_fn |}.
+
+(* component morphisms *)
+Definition msg_morph_p (e : entrypoint) : entrypoint_b := 
+    match e with 
+    | next _ => inr tt (* not upgrade functionality *)
+    | upgrade_fun s' => inl (upgrade_fun_b s') (*  *)
+    end.
+Definition state_morph_p : storage -> storage_b := (fun (x : storage) => {| s_b := x.(s) ; |}).
+Definition setup_morph_p : setup -> setup_b := (fun (x : setup) => {| s_b := x.(s) |}).
+Definition error_morph_p : error -> error_b := (fun (x : error) => x).
 
 (* the coherence results *)
-Lemma init_coherence : forall c ctx s, 
-    (init_result_transform state_morph error_morph) ((Blockchain.init C) c ctx s) = 
-    (Blockchain.init C_s) c ctx (setup_morph s).
-Proof. auto. Qed.
+Lemma init_coherence_p : 
+    init_coherence_prop C C_b 
+        setup_morph_p state_morph_p error_morph_p.
+Proof. unfold init_coherence_prop. auto. Qed.
 
-Lemma recv_coherence : forall c ctx st op_msg, 
-    (recv_result_transform state_morph error_morph) ((Blockchain.receive C) c ctx st op_msg) = 
-    (Blockchain.receive C_s) c ctx (state_morph st) (option_map msg_morph op_msg).
+Lemma recv_coherence_p : 
+    recv_coherence_prop C C_b 
+        msg_morph_p state_morph_p error_morph_p.
 Proof.
-    intros. cbn.
-    destruct op_msg; auto. 
-    destruct e; auto.
-Qed. 
+    unfold recv_coherence_prop.
+    intros.
+    unfold result_functor.
+    cbn.
+    destruct op_msg; cbn.
+    -   unfold msg_morph_p.
+        destruct e eqn:H_e.
+        +   now destruct st.
+        +   now unfold state_morph_p.
+    -   now unfold error_morph_p.
+Qed.
 
 (* construct the morphism *)
-Definition f_s : ContractMorphism C C_s := 
-    simple_cm msg_morph setup_morph state_morph error_morph init_coherence recv_coherence.
+Definition f_p : ContractMorphism C C_b := 
+    build_contract_morphism C C_b
+        (* the morphisms *)
+        setup_morph_p msg_morph_p state_morph_p error_morph_p 
+        (* coherence *)
+        init_coherence_p recv_coherence_p.
 
-(* TODO this is a problem -- you want all *reachable* states of the contract ... *)
-Theorem f_s_is_surj : is_surj_cm f_s.
-Proof.
-    unfold is_surj_cm. repeat split; unfold is_surj; intro x.
-    -   destruct x as [x s_s]. destruct x as [c ctx].
-        pose (s := {| n := 0 ; s := (fun _ : N => 0) |}).
-        exists (c, ctx, s).
-        cbn. unfold setup_morph. destruct s_s. 
-        reflexivity.
-    -   destruct x.
-        +   admit.
-        +   exists (Err 0). cbn. unfold error_morph. admit.
-    -   admit.
-    -   admit.
-Admitted.
+End Quotient.
 
-End Projection.
 
-Section MutableFunctionality.
-Context { Base : ChainBase }.
-
-(* contract types definition *)
-Definition setup_i := N.
-Inductive entrypoint_i := | next_i (u : unit).
-Record storage_i := build_storage_i { n_i : N ; }.
-Definition error_i := N.
-Definition result_i : Type := ResultMonad.result (storage_i * list ActionBody) error_i.
-
-(* derive serializable typeclass *)
-Section Serialization.
-    Global Instance storage_i_serializable : Serializable storage_i := todo "".
-    Global Instance entrypoint_i_serializable : Serializable entrypoint_i := todo "".
-End Serialization.
-
-(* init function definition *)
-Definition init_i (_ : Chain)
-                (_ : ContractCallContext)
-                (n : setup_i)
-                : ResultMonad.result storage_i N := 
-    let storage_i := {| n_i := n ; |} in 
-    Ok (storage_i).
-
-(* receive function definition *)
-Axiom s_next : N -> N.
-
-Definition receive_i (_ : Chain)
-                (_ : ContractCallContext)
-                (storage_i : storage_i)
-                (msg : option entrypoint_i)
-                : result_i :=
-    match msg with 
-    | Some (next_i _) => 
-        let st := {| n_i := s_next storage_i.(n_i) ; |} in 
-        Ok (st, [])
-    | None => Err 0
-    end.
-
-(* construct the contract *)
-Definition C_i : Contract setup_i entrypoint_i storage_i error_i := 
-    build_contract init_i receive_i.
-
-End MutableFunctionality.
-
+(** f_i : forall v, C_f v -> C *)
 Section Embedding.
-Context { Base : ChainBase }.
 
-(* using the simple morphism construction *)
-Definition msg_morph' (e : entrypoint_i) : entrypoint := 
+Definition msg_morph_i (v : storage_b) (e : entrypoint_f v) : entrypoint := 
     match e with 
-    | next_i _ => next tt
+    | next_f _ => next tt
     end.
-Definition setup_morph' (st_i : setup_i) : setup := {| 
-    n := st_i ; 
-    s := s_next ; |}.
-Definition state_morph' (st_i : storage_i) : storage := 
-    {| n := st_i.(n_i) ; s := s_next ; |}.
-Definition error_morph' : error_i -> error := id.
+Definition setup_morph_i (v : storage_b) (st_f : setup_f v) : setup := {| 
+    n := st_f ; 
+    s := s_b v ; |}.
+Definition state_morph_i (v : storage_b) (st_f : storage_f v) : storage := 
+    {| n := st_f.(n_f) ; s := s_b v ; |}.
+Definition error_morph_i (v : storage_b) : error_f v -> error := id.
 
 (* the coherence results *)
-Lemma init_coherence' : forall c ctx s, 
-    (init_result_transform state_morph' error_morph') ((Blockchain.init C_i) c ctx s) = 
-    (Blockchain.init C) c ctx (setup_morph' s).
-Proof. auto. Qed. 
+Lemma init_coherence_i (v : storage_b) : 
+    init_coherence_prop (C_f v) C (setup_morph_i v) (state_morph_i v) (error_morph_i v).
+Proof. unfold init_coherence_prop. auto. Qed. 
 
-Lemma recv_coherence' : forall c ctx st op_msg, 
-    (recv_result_transform state_morph' error_morph') ((Blockchain.receive C_i) c ctx st op_msg) = 
-    (Blockchain.receive C) c ctx (state_morph' st) (option_map msg_morph' op_msg).
+Lemma recv_coherence_i (v : storage_b) : 
+    recv_coherence_prop (C_f v) C (msg_morph_i v) (state_morph_i v) (error_morph_i v).
 Proof.
-    intros. cbn.
+    unfold recv_coherence_prop.
+    intros.
     destruct op_msg; auto.
-    destruct e; auto.
-Qed. 
+    now destruct e.
+Qed.
 
 (* construct the morphism *)
-Definition f_i : ContractMorphism C_i C := 
-    simple_cm msg_morph' setup_morph' state_morph' error_morph' init_coherence' recv_coherence'.
-
-Theorem f_s_is_inj : is_inj_cm f_s.
-Proof.
-    unfold is_inj_cm, is_inj. repeat split; intros.
-Admitted.
+Definition fi_param (v : storage_b) : ContractMorphism (C_f v) C := 
+    build_contract_morphism (C_f v) C 
+        (* the morphisms *)
+        (setup_morph_i v) (msg_morph_i v) (state_morph_i v) (error_morph_i v) 
+        (* coherence results *)
+        (init_coherence_i v) (recv_coherence_i v).
 
 End Embedding.
 
-Section UpgradeabilityThm.
 
-Theorem upgrade_mechanism : 
-    forall bstate caddr cstate msg s' cstate' acts chain ctx,
-    (* state is reachable *)
-    reachable bstate -> 
-    (* the contract address is caddr with state cstate *)
-    env_contracts bstate caddr = Some (C : WeakContract) -> 
-    contract_state bstate caddr = Some cstate -> 
-    (* a call to upgrade_fun was successful *)
-    msg = upgrade_fun s' ->  
-    receive C chain ctx cstate (Some msg) = Ok(cstate', acts) -> 
-    (* exists a contract C_i and an embedding *)
-    exists C_i (f_i : ContractMorphism C_i C), 
-    is_inj_cm f_i /\ 
-    (* with storage as desired *)
-    cstate' = 
-    (state_morph f_i) {| n := cstate'.(n) ; |}.    
+(** Here we prove the core result that the family of versioned contracts and the 
+    base contract given above provide an upgradeability decomposition of our contract C. *)
+Section UpgradeabilityDecomposition.
+Definition extract_version (m : entrypoint_skel) : storage_b := 
+    match m with | upgrade_fun_b s_b => {| s_b := s_b |} end.
+Definition new_version_state old_v msg (st : storage_f old_v) : storage_f (extract_version msg) := st.
+
+Theorem upgradeability_decomposition :
+    upgradeability_decomposition fi_param f_p extract_version new_version_state.
 Proof.
-Admitted.
+    unfold upgradeability_decomposition.
+    repeat split.
+    (* msg_required *)
+    -   unfold ContractMorphisms.msg_required. 
+        intros. 
+        now exists 0.
+    (* init_versioned *)
+    -   unfold init_versioned.
+        intros ? ? ? s init_ok.
+        destruct init_state as [n_i s_i].
+        unfold is_versioned.
+        now exists {| s_b := s_i |}, {| n_f := n_i |}.
+    (* msg_decomposable *)
+    (* -> *)
+    -   simpl.
+        intro H_null.
+        unfold msg_morph_p in H_null.
+        destruct m; try inversion H_null.
+        destruct u.
+        now exists (next_f tt).
+    (* <- *)
+    -   simpl.
+        intro H_preim.
+        unfold msg_morph_i in H_preim.
+        destruct H_preim as [m' H_preim].
+        destruct m'.
+        unfold msg_morph_p.
+        now destruct m; try inversion H_preim.
+    (* states categorized *)
+    (* -> *)
+    -   simpl.
+        intro H_preim.
+        destruct H_preim as [st_f H_preim].
+        destruct st_f as [nf].
+        unfold state_morph_i in H_preim.
+        simpl in H_preim.
+        destruct st as [n s].
+        now inversion H_preim.
+    (* <- *)
+    -   simpl.
+        unfold state_morph_p, state_morph_i.
+        destruct c_version as [sb], st as [n s].
+        cbn.
+        intro H.
+        inversion H.
+        now exists {| n_f := n |}.
+    (* version transition *)
+    -   unfold version_transition.
+        simpl.
+        unfold msg_morph_p, state_morph_i.
+        intros * H_cstate_preim ? ? ? ? ? ? recv_some is_upgrade_msg.
+        destruct msg; try inversion is_upgrade_msg.
+        inversion recv_some.
+        f_equal.
+        unfold new_version_state.
+        now rewrite H_cstate_preim.
+Qed.
 
+End UpgradeabilityDecomposition.
 
-Theorem upgradeability_invariance : 
-    forall bstate caddr cstate msg s' cstate' acts,
-    (* state is reachable *)
-    reachable bstate -> 
-    (* the contract address is caddr with state cstate *)
+End Morphisms.
+
+Section Decomposition.
+
+(** Theorem: all reachable contract states are versioned according to this indexing *)
+Theorem all_states_versioned : 
+    forall bstate caddr (trace : ChainTrace empty_state bstate),
+    (* where C is at caddr with state cstate, *)
     env_contracts bstate caddr = Some (C : WeakContract) -> 
-    contract_state bstate caddr = Some cstate -> 
-    (* exists a surjection onto C_s *)
-    exists (f_s : ContractMorphism C C_s).
-Proof. intros. exact f_s. Qed.
+    exists (cstate : storage),
+    contract_state bstate caddr = Some cstate /\
+    (* then every contract state cstate is versioned *)
+    is_versioned fi_param cstate.
+Proof.
+    intros * ? c_at_caddr.
+    pose proof (versioned_invariant fi_param f_p extract_version new_version_state bstate caddr trace c_at_caddr).
+    destruct H as [cstate [cstate_st versioned]].
+    exists cstate.
+    split; auto.
+    apply (versioned upgradeability_decomposition).
+Qed.
 
-End UpgradeabilityThm.
+(** Theorem: Versioning moves along as we've described it. *)
+Theorem upgrade_decomposed : 
+    (* Forall versioned contract states (incl. all reachable states), *)
+    forall cstate c_version cstate_f,
+    cstate = state_morph (C_f c_version) C (fi_param c_version) cstate_f ->
+    (* And forall calls to the versioned contract *)
+    forall chain ctx m new_state new_acts,
+    receive chain ctx cstate (Some m) = Ok (new_state, new_acts) -> 
+    (* the contract state either stays within this version *)
+    (exists cstate_f', new_state = state_morph (C_f c_version) C (fi_param c_version) cstate_f') \/
+    (* or it moves onto a new version as we've described it. *)
+    (exists c_version' cstate_f',
+    new_state = state_morph (C_f c_version') C (fi_param c_version') cstate_f').
+Proof.
+    intros * cstate_preim * recv_some.
+    apply (upgradeability_decomposed fi_param f_p extract_version new_version_state cstate c_version cstate_f upgradeability_decomposition cstate_preim chain ctx m new_state new_acts recv_some).
+Qed.
+
+End Decomposition.
+
+End Upgradeable.
