examples/contractMorphisms/upgradeable/UpgradeSpec.v
@@ -1,0 +1,137 @@
+From ConCert.Execution Require Import Blockchain.
+From ConCert.Execution Require Import Containers.
+From ConCert.Execution Require Import ContractCommon.
+From ConCert.Execution Require Import Monad.
+From ConCert.Execution Require Import ResultMonad.
+From ConCert.Execution Require Import Serializable.
+From ConCert.Execution Require Import ContractMorphisms.
+From ConCert.Execution Require Import ContractSystems.
+From ConCert.Utils Require Import RecordUpdate.
+From ConCert.Utils Require Import Extras.
+From Coq Require Import Ensembles.
+From Coq Require Import ZArith_base.
+From Coq Require Import QArith_base.
+From Coq Require Import String.
+From Coq Require Import List.
+From Coq Require Import Fin.
+From Coq.Init Require Import Byte.
+
+Import ListNotations.
+Open Scope N_scope.
+Open Scope string.
+
+
+(** Example 5.5.2: Mutable and Immutable Parts: Splitting an Upgradeable Contract 
+    This example ... TODO 
+
+*)
+
+Section UpgradeTheory.
+Context { Base : ChainBase }.
+
+Context `{Serializable Msg} `{Serializable Setup} `{Serializable State} `{Serializable Error}
+        `{Serializable Msg_fnct} `{Serializable Setup_fnct} 
+        `{Serializable State_fnct} `{Serializable Error_fnct}
+        `{Serializable Msg_base} `{Serializable Setup_base} 
+        `{Serializable State_base} `{Serializable Error_base}.
+
+(* I have three contracts: C, C_fnct, C_base *)
+Context 
+  (* C is the full contract *)
+  { C : Contract Setup Msg State Error } 
+  (* C_fnct is "current", non-upgradeable contract version/functionality *)
+  { C_fnct : Contract Setup_fnct Msg_fnct State_fnct Error_fnct }
+  (* C_skel is the skeleton/constant contract; we will sum this with null_contract *)
+  { C_skel : Contract Setup_base Msg_base State_base Error_base }.
+
+(*  *)
+Definition C_base := pointed_contract C_skel.
+
+(* We have an EMBEDDING of C_fnct into C *)
+Context { msg_morph_i : Msg_fnct -> Msg } 
+  { state_morph_i : State_fnct -> State }
+  { setup_morph_i : Setup_fnct -> Setup }
+  { error_morph_i : Error_fnct -> Error }
+  { msg_morph_i_inj : is_inj msg_morph_i } 
+  { state_morph_i_inj : is_inj state_morph_i }
+  { setup_morph_i_inj : is_inj setup_morph_i }.
+
+Definition Msg_base' := (Msg_base + unit)%type.
+
+(* We have a QUOTIENT of C_fnct onto C_base *)
+Context {msg_morph_p : Msg -> Msg_base'}
+  {state_morph_p : State -> State_base}
+  {setup_morph_p : Setup -> Setup_base}
+  {error_morph_p : Error -> Error_base}
+  {msg_morph_p_surj : is_surj msg_morph_p}
+  {state_morph_p_surj : is_surj state_morph_p}
+  {setup_morph_p_surj : is_surj setup_morph_p}.
+
+(* We have exact sequences on the message type *)
+Context { null_state : State_base } { null_setup : Setup_base }
+  { msg_exact : forall m,
+  msg_morph_p m = inr tt <-> 
+  (exists m', m = msg_morph_i m') }
+  { state_exact : forall st, 
+  state_morph_p st = null_state <->
+  (exists st', st = state_morph_i st')}
+  { setup_exact : forall s, 
+  setup_morph_p s = null_setup <->
+  (exists s', s = setup_morph_i s')}.
+
+
+
+(** This is an "exact sequence" of contracts: 
+    (null ->) C -> C_fnct ->> C_skel (-> null) *)
+
+(** Now we construct the morphisms. *)
+
+(* Construct the Embedding *)
+Context { init_coherence_i : init_coherence_prop C_fnct C setup_morph_i state_morph_i error_morph_i }
+        { recv_coherence_i : recv_coherence_prop C_fnct C msg_morph_i state_morph_i error_morph_i }.
+
+(* The Embedding *)
+Definition cm_embed : ContractMorphism C_fnct C := 
+    build_contract_morphism C_fnct C 
+      (* the morphisms *)
+      setup_morph_i msg_morph_i state_morph_i error_morph_i
+      (* coherence *)
+      init_coherence_i recv_coherence_i.
+
+(** Construct the Surjection *)
+Context { init_coherence_p : init_coherence_prop C C_base setup_morph_p state_morph_p error_morph_p }
+        { recv_coherence_p : recv_coherence_prop C C_base msg_morph_p state_morph_p error_morph_p }.
+
+(* The Surjection *)
+Definition cm_quot : ContractMorphism C C_base := 
+    build_contract_morphism C C_base
+      (* the morphisms *)
+      setup_morph_p msg_morph_p state_morph_p error_morph_p
+      (* coherence *)
+      init_coherence_p recv_coherence_p.
+
+(** Now we have an "exact" sequence of contracts. *)
+  
+(* A theorem that states that 
+    "every execution trace is either from C_fnct or conforms to C_base" *)
+Theorem exact_decompose : forall c ctx prev_state next_state new_acts msg, 
+  (* If receive C executes successfully with some msg, then ...  *)
+  receive C c ctx prev_state (Some msg) = Ok (next_state, new_acts) ->
+  (* EITHER prev_state and msg have preimages in C_f, or ... *)
+  (exists prev_state_f msg_f,
+    (* msg is coming from one or the other *)
+    msg = msg_morph_i msg_f /\
+    (* for which coherence holds, prob not this *)
+    prev_state = state_morph_i prev_state_f /\
+    (* and the images of each are uninteresting in C_base *)
+    state_morph_p prev_state = null_state /\
+    msg_morph_p msg = inr tt) \/
+  (* OR the image in C_b is nontrivial *)
+  (exists m,
+    state_morph_p prev_state <> null_state /\
+    msg_morph_p msg = inl m).
+Proof.
+Admitted.
+
+
+End UpgradeTheory.
