Makefile
@@ -2,8 +2,8 @@ all: concert theory
 .PHONY: all
 
 concert:
-	+@make -C phd-thesis-ConCert/utils
-	+@make -C phd-thesis-ConCert/execution
+	+@make -C FinCert-ConCert-fork/utils
+	+@make -C FinCert-ConCert-fork/execution
 .PHONY: concert
 
 CoqMakefile: _CoqProject
@@ -15,8 +15,8 @@ theory: concert CoqMakefile
 
 clean: CoqMakefile
 	+@make -f CoqMakefile clean
-	+@make -C phd-thesis-ConCert/utils clean
-	+@make -C phd-thesis-ConCert/execution clean
+	+@make -C FinCert-ConCert-fork/utils clean
+	+@make -C FinCert-ConCert-fork/execution clean
 	rm -f CoqMakefile
 .PHONY: clean
 
@@ -40,16 +40,16 @@ html: all
 	rm -rf docs
 	mkdir docs
 	coqdoc --html --interpolate --parse-comments \
-		--with-header phd-thesis-ConCert/extra/header.html --with-footer phd-thesis-ConCert/extra/footer.html \
+		--with-header FinCert-ConCert-fork/extra/header.html --with-footer FinCert-ConCert-fork/extra/footer.html \
 		--toc \
 		--external https://plv.mpi-sws.org/coqdoc/stdpp stdpp \
 		--external https://metacoq.github.io/html MetaCoq \
 		--external https://coq-community.org/coq-ext-lib/v0.11.7 ExtLib \
 		-R theories/custodian ConCert.x4c.Custodian \
 		-R theories/fa2 ConCert.x4c.FA2 \
-		-d docs `find . -type f \( -wholename "*theories/*" \) -name "*.v" ! -wholename "./phd-thesis-ConCert/*" ! -wholename "./_opam/*"`
-	cp phd-thesis-ConCert/extra/resources/coqdocjs/*.js docs
-	cp phd-thesis-ConCert/extra/resources/coqdocjs/*.css docs
-	cp phd-thesis-ConCert/extra/resources/toc/*.js docs
-	cp phd-thesis-ConCert/extra/resources/toc/*.css docs
+		-d docs `find . -type f \( -wholename "*theories/*" \) -name "*.v" ! -wholename "./FinCert-ConCert-fork/*" ! -wholename "./_opam/*"`
+	cp FinCert-ConCert-fork/extra/resources/coqdocjs/*.js docs
+	cp FinCert-ConCert-fork/extra/resources/coqdocjs/*.css docs
+	cp FinCert-ConCert-fork/extra/resources/toc/*.js docs
+	cp FinCert-ConCert-fork/extra/resources/toc/*.css docs
 .PHONY: html
