README.md
@@ -1,6 +1,6 @@
 # Formal Verification of Financial Smart Contracts
 
-This repository is one of two that houses the code of my PhD thesis, the other being my [fork of ConCert](https://github.com/differentialderek/phd-thesis-ConCert-fork), which is imported as a Git submodule.
+This repository is one of two that houses the code of my PhD thesis, the other being my [fork of ConCert](https://github.com/differentialderek/FinCert-ConCert-fork/tree/contract_morphisms), which is imported as a Git submodule.
 This repository is designed to be self-contained, but can also be used as a companion to the text of my thesis, [which can be found here](thesis.pdf).
 
 The goal of this repository is to build up theories and tools for reasoning rigorously about financial smart contracts. We introduce various new notions to reasoning about contracts, including:
@@ -17,12 +17,12 @@ Using these techniques we can reason about:
 
 Clone the repository with the `--recursive` tag so that you include the submodule.
 ```
-git clone git@github.com:differentialderek/phd-thesis.git --recursive
+git clone git@github.com:differentialderek/FinCert.git --recursive
 ```
 
-Go into the `phd-thesis-ConCert/` subdirectory, my fork of the ConCert codebase, and follow the [install instructions there](https://github.com/differentialderek/phd-thesis-ConCert-fork/tree/ab15ded163e630bad9ef74a0ff7ac5ce2c52171c). Note that installation may take some time.
+Go into the `FinCert-ConCert-fork/` subdirectory, my fork of the ConCert codebase, and follow the [install instructions there](https://github.com/differentialderek/FinCert-ConCert-fork/tree/contract_morphisms). Note that installation may take some time, and make sure you're on the `contract_morphisms` branch.
 
-Now go back to the root `phd-thesis/` directory, and make the Coq project.
+Now go back to the root `FinCert/` directory, and make the Coq project.
 ```
 make
 ```
@@ -38,7 +38,7 @@ For VSCode users, `VSCoq` seems to work well as a plugin with which to step thro
 ## Organization 
 
 * the `specifications` folder houses various formalized specifications, including of structured pools, token contracts, and AMMs
-* the `phd-thesis-ConCert` folder, the reasoning enginge of the repository, is a fork of ConCert with modifications to include contract morphisms and equivalences of contracts (including bisimulations)
+* the `FinCert-ConCert-fork` folder, the reasoning enginge of the repository, is a fork of ConCert with modifications to include contract morphisms and equivalences of contracts (including bisimulations)
 * the `examples` folder houses examples of using the techniques mentioned above in verifying smart contracts
 * the `implementations` folder is to house formally verified implementations of, *e.g.* token or AMM contracts (currently empty)
 * the `theories` folder is to house theories, *e.g.* a theory of DeFi, built on top of ConCert (currently empty)
