examples/README.md
@@ -1,3 +1,6 @@
 # Example Directory
 
-This is a directory for examples of using various meta-theoretic tools, such as contract morphisms and equivalences, in proof and specification of smart contracts.
+We introduce various theoretical tools for the purpose of reasoning about complex properties of financial smart contracts and their specifications.
+
+This is a directory houses various examples of using these tools, such as contract morphisms and equivalences, in proof and specification of smart contracts.
+
