examples/contractMorphisms/optimizing/README.md
@@ -1,0 +1,5 @@
+# Contract Optimization
+
+TODO
+
+This is probably actually an example of weakly equivalent contracts! Those that induce bisimulations of chains but *not* isomorphisms of contracts!
