examples/contractSystems/directSum.v
@@ -1,0 +1,1 @@
+(* an example of a direct sum of contracts, and a weak equivalence *)
